---
title:  Proposition 7
subtitle: 
author:
routes:
  aliases:
    - /elem.7.7
collection:
  name: elements
  showCount: true
  showMenu: true
content:
  items: '@self.children'
child_type: article
figure:
  image:
  alt:
  title:
  caption:
taxonomy:
  tag:
  category:
    - 
---

<p>
       <hi rend="ital">If a number be that part of a number, which a number subtracted is of a number subtracted, the remainder will also be the same part of the remainder that the whole is of the whole.</hi>
      </p>

===

<h1>PROPOSITION 7.</h1>
<p>
       <span class="ital">If a number be that part of a number, which a number subtracted is of a number subtracted, the remainder will also be the same part of the remainder that the whole is of the whole.</span>
      </p>

<p>For let the number <span class="ital">AB</span> be that part of the number <span class="ital">CD</span> which <span class="ital">AE</span> subtracted is of <span class="ital">CF</span> subtracted; I say that the remainder <span class="ital">EB</span> is also the same part of the remainder <span class="ital">FD</span> that the whole <span class="ital">AB</span> is of the whole <span class="ital">CD</span>. 
      </p>

<p>For, whatever part <span class="ital">AE</span> is of <span class="ital">CF</span>, the same part also let <span class="ital">EB</span> be of <span class="ital">CG</span>. </p>

<p>Now since, whatever part <span class="ital">AE</span> is of <span class="ital">CF</span>, the same part also is <span class="ital">EB</span> of <span class="ital">CG</span>, therefore, whatever part <span class="ital">AE</span> is of <span class="ital">CF</span>, the same part also is <span class="ital">AB</span> of <span class="ital">GF</span>. [<a href="/elem.7.5">VII. 5</a>] </p>

<p>But, whatever part <span class="ital">AE</span> is of <span class="ital">CF</span>, the same part also, by hypothesis, is <span class="ital">AB</span> of <span class="ital">CD</span>; therefore, whatever part <span class="ital">AB</span> is of <span class="ital">GF</span>, the same part is it of <span class="ital">CD</span> also; therefore <span class="ital">GF</span> is equal to <span class="ital">CD</span>. </p>

<p>Let <span class="ital">CF</span> be subtracted from each; therefore the remainder <span class="ital">GC</span> is equal to the remainder <span class="ital">FD</span>. </p>

<p>Now since, whatever part <span class="ital">AE</span> is of <span class="ital">CF</span>, the same part also is <span class="ital">EB</span> of <span class="ital">GC</span>, while <span class="ital">GC</span> is equal to <span class="ital">FD</span>, therefore, whatever part <span class="ital">AE</span> is of <span class="ital">CF</span>, the same part also is <span class="ital">EB</span> of <span class="ital">FD</span>. </p>

<p>But, whatever part <span class="ital">AE</span> is of <span class="ital">CF</span>, the same part also is <span class="ital">AB</span> of <span class="ital">CD</span>; <pb n="307"/>therefore also the remainder <span class="ital">EB</span> is the same part of the remainder <span class="ital">FD</span> that the whole <span class="ital">AB</span> is of the whole <span class="ital">CD</span>. Q. E. D.</p>
