---
title:  Proposition 9.3
subtitle: 
author:
routes:
  aliases:
    - /elem.9.3
collection:
  name: elements
  showCount: true
  showMenu: true
content:
  items: '@self.children'
child_type: article
figure:
  image:
  alt:
  title:
  caption:
taxonomy:
  tag:
  category:
    - 
---

<p>
       <hi rend="ital">If a cube number by multiplying itself make some number, the product will be cube.</hi>
      </p>

===

<h1>PROPOSITION 3.</h1>
<p>
       <span class="ital">If a cube number by multiplying itself make some number, the product will be cube.</span>
      </p>

<p>For let the cube number <span class="ital">A</span> by multiplying itself make <span class="ital">B</span>; I say that <span class="ital">B</span> is cube. <pb n="386"/></p>

<p>For let <span class="ital">C</span>, the side of <span class="ital">A</span>, be taken, and let <span class="ital">C</span> by multiplying itself make <span class="ital">D</span>. </p>

<p>It is then manifest that <span class="ital">C</span> by multiplying <span class="ital">D</span> has made <span class="ital">A</span>. 
      </p>

<p>Now, since <span class="ital">C</span> by multiplying itself has made <span class="ital">D</span>, therefore <span class="ital">C</span> measures <span class="ital">D</span> according to the units in itself. </p>

<p>But further the unit also measures <span class="ital">C</span> according to the units in it; therefore, as the unit is to <span class="ital">C</span>, so is <span class="ital">C</span> to <span class="ital">D</span>. [<a href="/elem.7.def.20">VII. Def. 20</a>] </p>

<p>Again, since <span class="ital">C</span> by multiplying <span class="ital">D</span> has made <span class="ital">A</span>, therefore <span class="ital">D</span> measures <span class="ital">A</span> according to the units in <span class="ital">C</span>. </p>

<p>But the unit also measures <span class="ital">C</span> according to the units in it; therefore, as the unit is to <span class="ital">C</span>, so is <span class="ital">D</span> to <span class="ital">A</span>. </p>

<p>But, as the unit is to <span class="ital">C</span>, so is <span class="ital">C</span> to <span class="ital">D</span>; therefore also, as the unit is to <span class="ital">C</span>, so is <span class="ital">C</span> to <span class="ital">D</span>, and <span class="ital">D</span> to <span class="ital">A</span>. </p>

<p>Therefore between the unit and the number <span class="ital">A</span> two mean proportional numbers <span class="ital">C</span>, <span class="ital">D</span> have fallen in continued proportion. </p>

<p>Again, since <span class="ital">A</span> by multiplying itself has made <span class="ital">B</span>, therefore <span class="ital">A</span> measures <span class="ital">B</span> according to the units in itself. </p>

<p>But the unit also measures <span class="ital">A</span> according to the units in it; therefore, as the unit is to <span class="ital">A</span>, so is <span class="ital">A</span> to <span class="ital">B</span>. [<a href="/elem.7.def.20">VII. Def. 20</a>] </p>

<p>But between the unit and <span class="ital">A</span> two mean proportional numbers have fallen; therefore two mean proportional numbers will also fall between <span class="ital">A</span>, <span class="ital">B</span>. [<a href="/elem.8.8">VIII. 8</a>] </p>

<p>But, if two mean proportional numbers fall between two numbers, and the first be cube, the second will also be cube. [<a href="/elem.8.23">VIII. 23</a>] </p>

<p>And <span class="ital">A</span> is cube; therefore <span class="ital">B</span> is also cube. Q. E. D.</p>
