---
title:  Proposition 10.53
subtitle: 
author:
routes:
  aliases:
    - /elem.10.53
collection:
  name: elements
  showCount: true
  showMenu: true
content:
  items: '@self.children'
child_type: article
figure:
  image:
  alt:
  title:
  caption:
taxonomy:
  tag:
  category:
    - 
---

<p>
       <hi rend="ital">To find the sixth binomial straight line.</hi>
      </p>

===

<p>
       <span class="ital">To find the sixth binomial straight line.</span>
      </p>

<p>Let two numbers <span class="ital">AC</span>, <span class="ital">CB</span> be set out such that <span class="ital">AB</span> has not to either of them the ratio which a square number has to a square number; and let there also be another number <span class="ital">D</span> which is not square and which has not to either of the numbers <span class="ital">BA</span>, <span class="ital">AC</span> the ratio which a square number has to a square number. 
      </p>

<p>Let any rational straight line <span class="ital">E</span> be set out, and let it be contrived that, as <span class="ital">D</span> is to <span class="ital">AB</span>, so is the square on <span class="ital">E</span> to the square on <span class="ital">FG</span>; [<a href="/elem.10.6.p.1">X. 6, Por.</a>] therefore the square on <span class="ital">E</span> is commensurable with the square on <span class="ital">FG</span>. [<a href="/elem.10.6">X. 6</a>] </p>

<p>And <span class="ital">E</span> is rational; therefore <span class="ital">FG</span> is also rational. </p>

<p>Now, since <span class="ital">D</span> has not to <span class="ital">AB</span> the ratio which a square number has to a square number, <pb n="113"/>neither has the square on <span class="ital">E</span> to the square on <span class="ital">FG</span> the ratio which a square number has to a square number; therefore <span class="ital">E</span> is incommensurable in length with <span class="ital">FG</span>. [<a href="/elem.10.9">X. 9</a>] </p>

<p>Again, let it be contrived that, as <span class="ital">BA</span> is to <span class="ital">AC</span>, so is the square on <span class="ital">FG</span> to the square on <span class="ital">GH</span>. [<a href="/elem.10.6.p.1">X. 6, Por.</a>] </p>

<p>Therefore the square on <span class="ital">FG</span> is commensurable with the square on <span class="ital">HG</span>. [<a href="/elem.10.6">X. 6</a>] </p>

<p>Therefore the square on <span class="ital">HG</span> is rational; therefore <span class="ital">HG</span> is rational. </p>

<p>And, since <span class="ital">BA</span> has not to <span class="ital">AC</span> the ratio which a square number has to a square number, neither has the square on <span class="ital">FG</span> to the square on <span class="ital">GH</span> the ratio which a square number has to a square number; therefore <span class="ital">FG</span> is incommensurable in length with <span class="ital">GH</span>. [<a href="/elem.10.9">X. 9</a>] </p>

<p>Therefore <span class="ital">FG</span>, <span class="ital">GH</span> are rational straight lines commensurable in square only; therefore <span class="ital">FH</span> is binomial. [<a href="/elem.10.36">X. 36</a>] </p>

<p>It is next to be proved that it is also a sixth binomial straight line. </p>

<p>For since, as <span class="ital">D</span> is to <span class="ital">AB</span>, so is the square on <span class="ital">E</span> to the square on <span class="ital">FG</span>, and also, as <span class="ital">BA</span> is to <span class="ital">AC</span>, so is the square on <span class="ital">FG</span> to the square on <span class="ital">GH</span>, therefore, <foreign lang="la">ex aequali</foreign>, as <span class="ital">D</span> is to <span class="ital">AC</span>, so is the square on <span class="ital">E</span> to the square on <span class="ital">GH</span>. [<a href="/elem.5.22">V. 22</a>] </p>

<p>But <span class="ital">D</span> has not to <span class="ital">AC</span> the ratio which a square number has to a square number; therefore neither has the square on <span class="ital">E</span> to the square on <span class="ital">GH</span> the ratio which a square number has to a square number; therefore <span class="ital">E</span> is incommensurable in length with <span class="ital">GH</span>. [<a href="/elem.10.9">X. 9</a>] </p>

<p>But it was also proved incommensurable with <span class="ital">FG</span>; therefore each of the straight lines <span class="ital">FG</span>, <span class="ital">GH</span> is incommensurable in length with <span class="ital">E</span>. </p>

<p>And, since, as <span class="ital">BA</span> is to <span class="ital">AC</span>, so is the square on <span class="ital">FG</span> to the square on <span class="ital">GH</span>, therefore the square on <span class="ital">FG</span> is greater than the square on <span class="ital">GH</span>. </p>

<p>Let then the squares on <span class="ital">GH</span>, <span class="ital">K</span> be equal to the square on <span class="ital">FG</span>; <pb n="114"/>therefore, <foreign lang="la">convertendo</foreign>, as <span class="ital">AB</span> is to <span class="ital">BC</span>, so is the square on <span class="ital">FG</span> to the square on <span class="ital">K</span>. [<a href="/elem.5.19.p.1">V. 19, Por.</a>] </p>

<p>But <span class="ital">AB</span> has not to <span class="ital">BC</span> the ratio which a square number has to a square number; so that neither has the square on <span class="ital">FG</span> to the square on <span class="ital">K</span> the ratio which a square number has to a square number. </p>

<p>Therefore <span class="ital">FG</span> is incommensurable in length with <span class="ital">K</span>; [<a href="/elem.10.9">X. 9</a>] therefore the square on <span class="ital">FG</span> is greater than the square on <span class="ital">GH</span> by the square on a straight line incommensurable with <span class="ital">FG</span>. </p>

<p>And <span class="ital">FG</span>, <span class="ital">GH</span> are rational straight lines commensurable in square only, and neither of them is commensurable in length with the rational straight line <span class="ital">E</span> set out. </p>

<p>Therefore <span class="ital">FH</span> is a sixth binomial straight line. Q. E. D.
 </p>
<div id="elem.10.53.l.1" class="lemma">
       <h1>LEMMA.</h1>
       
<p>Let there be two squares <span class="ital">AB</span>, <span class="ital">BC</span>, and let them be placed so that <span class="ital">DB</span> is in a straight line with <span class="ital">BE</span>; therefore <span class="ital">FB</span> is also in a straight line with <span class="ital">BG</span>. </p>

       
<p>Let the parallelogram <span class="ital">AC</span> be completed; I say that <span class="ital">AC</span> is a square, that <span class="ital">DG</span> is a mean proportional between <span class="ital">AB</span>, <span class="ital">BC</span>, and further that <span class="ital">DC</span> is a mean proportional between <span class="ital">AC</span>, <span class="ital">CB</span>. 
       </p>

       
<p>For, since <span class="ital">DB</span> is equal to <span class="ital">BF</span>, and <span class="ital">BE</span> to <span class="ital">BG</span>, therefore the whole <span class="ital">DE</span> is equal to the whole <span class="ital">FG</span>. </p>

       
<p>But <span class="ital">DE</span> is equal to each of the straight lines <span class="ital">AH</span>, <span class="ital">KC</span>, and <span class="ital">FG</span> is equal to each of the straight lines <span class="ital">AK</span>, <span class="ital">HC</span>; [<a href="/elem.1.34">I. 34</a>] <pb n="116"/>therefore each of the straight lines <span class="ital">AH</span>, <span class="ital">KC</span> is also equal to each of the straight lines <span class="ital">AK</span>, <span class="ital">HC</span>. </p>

       
<p>Therefore the parallelogram <span class="ital">AC</span> is equilateral. </p>

       
<p>And it is also rectangular; therefore <span class="ital">AC</span> is a square. </p>

       
<p>And since, as <span class="ital">FB</span> is to <span class="ital">BG</span>, so is <span class="ital">DB</span> to <span class="ital">BE</span>, while, as <span class="ital">FB</span> is to <span class="ital">BG</span>, so is <span class="ital">AB</span> to <span class="ital">DG</span>, and, as <span class="ital">DB</span> is to <span class="ital">BE</span>, so is <span class="ital">DG</span> to <span class="ital">BC</span>, [<a href="/elem.6.1">VI. 1</a>] therefore also, as <span class="ital">AB</span> is to <span class="ital">DG</span>, so is <span class="ital">DG</span> to <span class="ital">BC</span>. [<a href="/elem.5.11">V. 11</a>] </p>

       
<p>Therefore <span class="ital">DG</span> is a mean proportional between <span class="ital">AB</span>, <span class="ital">BC</span>. </p>

       
<p>I say next that <span class="ital">DC</span> is also a mean proportional between <span class="ital">AC</span>, <span class="ital">CB</span>. </p>

       
<p>For since, as <span class="ital">AD</span> is to <span class="ital">DK</span>, so is <span class="ital">KG</span> to <span class="ital">GC</span>— for they are equal respectively— and, <foreign lang="la">componendo</foreign>, as <span class="ital">AK</span> is to <span class="ital">KD</span>, so is <span class="ital">KC</span> to <span class="ital">CG</span>, [<a href="/elem.5.18">V. 18</a>] while, as <span class="ital">AK</span> is to <span class="ital">KD</span>, so is <span class="ital">AC</span> to <span class="ital">CD</span>, and, as <span class="ital">KC</span> is to <span class="ital">CG</span>, so is <span class="ital">DC</span> to <span class="ital">CB</span>, [<a href="/elem.6.1">VI. 1</a>] therefore also, as <span class="ital">AC</span> is to <span class="ital">DC</span>, so is <span class="ital">DC</span> to <span class="ital">BC</span>. [<a href="/elem.5.11">V. 11</a>] </p>

       
<p>Therefore <span class="ital">DC</span> is a mean proportional between <span class="ital">AC</span>, <span class="ital">CB</span>. <span class="center">Being what it was proposed to prove.</span></p>

      </div>
