---
title:  Proposition 7.19
subtitle: 
author:
routes:
  aliases:
    - /elem.7.19
collection:
  name: elements
  showCount: true
  showMenu: true
content:
  items: '@self.children'
child_type: article
figure:
  image:
  alt:
  title:
  caption:
taxonomy:
  tag:
  category:
    - 
---

<p>
       <hi rend="ital">If four numbers be proportional, the number produced from the first and fourth will be equal to the number produced from the second and third; and, if the number produced from the first and fourth be equal to that produced from the second and third, the four numbers will be proportional.</hi>
      </p>

===

<p>
       <span class="ital">If four numbers be proportional, the number produced from the first and fourth will be equal to the number produced from the second and third; and, if the number produced from the first and fourth be equal to that produced from the second and third, the four numbers will be proportional.</span>
      </p>

<p>Let <span class="ital">A</span>, <span class="ital">B</span>, <span class="ital">C</span>, <span class="ital">D</span> be four numbers in proportion, so that, <span class="center">as <span class="ital">A</span> is to <span class="ital">B</span>, so is <span class="ital">C</span> to <span class="ital">D</span>;</span> and let <span class="ital">A</span> by multiplying <span class="ital">D</span> make <span class="ital">E</span>, and let <span class="ital">B</span> by multiplying <span class="ital">C</span> make <span class="ital">F</span>; I say that <span class="ital">E</span> is equal to <span class="ital">F</span>. </p>

<p>For let <span class="ital">A</span> by multiplying <span class="ital">C</span> make <span class="ital">G</span>. <pb n="319"/></p>

<p>Since, then, <span class="ital">A</span> by multiplying <span class="ital">C</span> has made <span class="ital">G</span>, and by multiplying <span class="ital">D</span> has made <span class="ital">E</span>, the number <span class="ital">A</span> by multiplying the two numbers <span class="ital">C</span>, <span class="ital">D</span> has made <span class="ital">G</span>, <span class="ital">E</span>. </p>

<p>Therefore, as <span class="ital">C</span> is to <span class="ital">D</span>, so is <span class="ital">G</span> to <span class="ital">E</span>. [<a href="/elem.7.17">VII. 17</a>] </p>

<p>But, as <span class="ital">C</span> is to <span class="ital">D</span>, so is <span class="ital">A</span> to <span class="ital">B</span>; therefore also, as <span class="ital">A</span> is to <span class="ital">B</span>, so is <span class="ital">G</span> to <span class="ital">E</span>. 
      </p>

<p>Again, since <span class="ital">A</span> by multiplying <span class="ital">C</span> has made <span class="ital">G</span>, but, further, <span class="ital">B</span> has also by multiplying <span class="ital">C</span> made <span class="ital">F</span>, the two numbers <span class="ital">A</span>, <span class="ital">B</span> by multiplying a certain number <span class="ital">C</span> have made <span class="ital">G</span>, <span class="ital">F</span>. </p>

<p>Therefore, as <span class="ital">A</span> is to <span class="ital">B</span>, so is <span class="ital">G</span> to <span class="ital">F</span>. [<a href="/elem.7.18">VII. 18</a>] </p>

<p>But further, as <span class="ital">A</span> is to <span class="ital">B</span>, so is <span class="ital">G</span> to <span class="ital">E</span> also; therefore also, as <span class="ital">G</span> is to <span class="ital">E</span>, so is <span class="ital">G</span> to <span class="ital">F</span>. </p>

<p>Therefore <span class="ital">G</span> has to each of the numbers <span class="ital">E</span>, <span class="ital">F</span> the same ratio; <span class="center">therefore <span class="ital">E</span> is equal to <span class="ital">F</span>. [cf. <a href="/elem.5.9">V. 9</a>]</span>
      </p>

<p>Again, let <span class="ital">E</span> be equal to <span class="ital">F</span>; I say that, as <span class="ital">A</span> is to <span class="ital">B</span>, so is <span class="ital">C</span> to <span class="ital">D</span>. </p>

<p>For, with the same construction, since <span class="ital">E</span> is equal to <span class="ital">F</span>, therefore, as <span class="ital">G</span> is to <span class="ital">E</span>, so is <span class="ital">G</span> to <span class="ital">F</span>. [cf. <a href="/elem.5.7">V. 7</a>] </p>

<p>But, as <span class="ital">G</span> is to <span class="ital">E</span>, so is <span class="ital">C</span> to <span class="ital">D</span>, [<a href="/elem.7.17">VII. 17</a>] <span class="center">and, as <span class="ital">G</span> is to <span class="ital">F</span>, so is <span class="ital">A</span> to <span class="ital">B</span>. [<a href="/elem.7.18">VII. 18</a>]</span>
      </p>

<p>Therefore also, as <span class="ital">A</span> is to <span class="ital">B</span>, so is <span class="ital">C</span> to <span class="ital">D</span>. Q. E. D.</p>
