---
title:  Proposition 12.5
subtitle: 
author:
routes:
  aliases:
    - /elem.12.5
collection:
  name: elements
  showCount: true
  showMenu: true
content:
  items: '@self.children'
child_type: article
figure:
  image:
  alt:
  title:
  caption:
taxonomy:
  tag:
  category:
    - 
---

<p>
       <hi rend="ital">Pyramids which are of the same height and have triangular bases are to one another as the bases.</hi>
      </p>

===

<p>
       <span class="ital">Pyramids which are of the same height and have triangular bases are to one another as the bases.</span>
      </p>

<p>Let there be pyramids of the same height, of which the triangles <span class="ital">ABC</span>, <span class="ital">DEF</span> are the bases and the points <span class="ital">G</span>, <span class="ital">H</span> the vertices; I say that, as the base <span class="ital">ABC</span> is to the base <span class="ital">DEF</span>, so is the pyramid <span class="ital">ABCG</span> to the pyramid <span class="ital">DEFH</span>. 
      </p>

<p>For, if the pyramid <span class="ital">ABCG</span> is not to the pyramid <span class="ital">DEFH</span> as the base <span class="ital">ABC</span> is to the base <span class="ital">DEF</span>, then, as the base <span class="ital">ABC</span> is to the base <span class="ital">DEF</span>, so will the pyramid <span class="ital">ABCG</span> be either to some solid less than the pyramid <span class="ital">DEFH</span> or to a greater. </p>

<p>Let it, first, be in that ratio to a less solid <span class="ital">W</span>, and let the pyramid <span class="ital">DEFH</span> be divded into two pyramids equal to one another and similar to the whole and into two equal prisms; then the two prisms are greater than the half of the whole pyramid. [<a href="/elem.12.3">XII. 3</a>] <pb n="387"/></p>

<p>Again, let the pyramids arising from the divsion be similarly divded, and let this be done continually until there are left over from the pyramid <span class="ital">DEFH</span> some pyramids which are less than the excess by which the pyramid <span class="ital">DEFH</span> exceeds the solid <span class="ital">W</span>. [X. I] </p>

<p>Let such be left, and let them be, for the sake of argument, <span class="ital">DQRS</span>, <span class="ital">STUH</span>; therefore the remainders, the prisms in the pyramid <span class="ital">DEFH</span>, are greater than the solid <span class="ital">W</span>. </p>

<p>Let the pyramid <span class="ital">ABCG</span> also be divded similarly, and a similar number of times, with the pyramid <span class="ital">DEFH</span>; therefore, as the base <span class="ital">ABC</span> is to the base <span class="ital">DEF</span>, so are the prisms in the pyramid <span class="ital">ABCG</span> to the prisms in the pyramid <span class="ital">DEFH</span>. [<a href="/elem.12.4">XII. 4</a>] </p>

<p>But, as the base <span class="ital">ABC</span> is to the base <span class="ital">DEF</span>, so also is the pyramid <span class="ital">ABCG</span> to the solid <span class="ital">W</span>; therefore also, as the pyramid <span class="ital">ABCG</span> is to the solid <span class="ital">W</span>, so are the prisms in the pyramid <span class="ital">ABCG</span> to the prisms in the pyramid <span class="ital">DEFH</span>; [V. II] therefore, alternately, as the pyramid <span class="ital">ABCG</span> is to the prisms in it, so is the solid <span class="ital">W</span> to the prisms in the pyramid <span class="ital">DEFH</span>. [<a href="/elem.5.16">V. 16</a>] </p>

<p>But the pyramid <span class="ital">ABCG</span> is greater than the prisms in it; therefore the solid <span class="ital">W</span> is also greater than the prisms in the pyramid <span class="ital">DEFH</span>. </p>

<p>But it is also less: which is impossible. </p>

<p>Therefore the prism <span class="ital">ABCG</span> is not to any solid less than the pyramid <span class="ital">DEFH</span> as the base <span class="ital">ABC</span> is to the base <span class="ital">DEF</span>. </p>

<p>Similarly it can be proved that neither is the pyramid <span class="ital">DEFH</span> to any solid less than the pyramid <span class="ital">ABCG</span> as the base <span class="ital">DEF</span> is to the base <span class="ital">ABC</span>. </p>

<p>I say next that neither is the pyramid <span class="ital">ABCG</span> to any solid greater than the pyramid <span class="ital">DEFH</span> as the base <span class="ital">ABC</span> is to the base <span class="ital">DEF</span>. </p>

<p>For, if possible, let it be in that ratio to a greater solid <span class="ital">W</span>; therefore, inversely, as the base <span class="ital">DEF</span> is to the base <span class="ital">ABC</span>, so is the solid <span class="ital">W</span> to the pyramid <span class="ital">ABCG</span>. <pb n="388"/></p>

<p>But, as the solid <span class="ital">W</span> is to the solid <span class="ital">ABCG</span>, so is the pyramid <span class="ital">DEFH</span> to some solid less than the pyramid <span class="ital">ABCG</span>, as was before proved; [<a href="/elem.12.2.l.1">XII. 2, Lemma</a>] therefore also, as the base <span class="ital">DEF</span> is to the base <span class="ital">ABC</span>, so is the pyramid <span class="ital">DEFH</span> to some solid less than the pyramid <span class="ital">ABCG</span>: [V. II] which was proved absurd. </p>

<p>Therefore the pyramid <span class="ital">ABCG</span> is not to any solid greater than the pyramid <span class="ital">DEFH</span> as the base <span class="ital">ABC</span> is to the base <span class="ital">DEF</span>. </p>

<p>But it was proved that neither is it in that ratio to a less solid. </p>

<p>Therefore, as the base <span class="ital">ABC</span> is to the base <span class="ital">DEF</span>, so is the pyramid <span class="ital">ABCG</span> to the pyramid <span class="ital">DEFH</span>. Q. E. D.</p>
