---
title:  Proposition 12.12
subtitle: 
author:
routes:
  aliases:
    - /elem.12.12
collection:
  name: elements
  showCount: true
  showMenu: true
content:
  items: '@self.children'
child_type: article
figure:
  image:
  alt:
  title:
  caption:
taxonomy:
  tag:
  category:
    - 
---

<p>
       <hi rend="ital">Similar cones and cylinders are to one another in the triplicate ratio of the diameters in their bases.</hi>
      </p>

===

<p>
       <span class="ital">Similar cones and cylinders are to one another in the triplicate ratio of the diameters in their bases.</span>
      </p>

<p>Let there be similar cones and cylinders, let the circles <span class="ital">ABCD</span>, <span class="ital">EFGH</span> be their bases, <span class="ital">BD</span>, <span class="ital">FH</span> the diameters of the bases, and <span class="ital">KL</span>, <span class="ital">MN</span> the axes of the cones and cylinders; I say that the cone of which the circle <span class="ital">ABCD</span> is the base and the point <span class="ital">L</span> the vertex has to the cone of which the circle <span class="ital">EFGH</span> is the base and the point <span class="ital">N</span> the vertex the ratio triplicate of that which <span class="ital">BD</span> has to <span class="ital">FH</span>. 
      </p>

<p>For, if the cone <span class="ital">ABCDL</span> has not to the cone <span class="ital">EFGHN</span> the ratio triplicate of that which <span class="ital">BD</span> has to <span class="ital">FH</span>, the cone <span class="ital">ABCDL</span> will have that triplicate ratio either to some solid less than the cone <span class="ital">EFGHN</span> or to a greater. </p>

<p>First, let it have that triplicate ratio to a less solid <span class="ital">O</span>. </p>

<p>Let the square <span class="ital">EFGH</span> be inscribed in the circle <span class="ital">EFGH</span>; [<a href="/elem.4.6">IV. 6</a>] therefore the square <span class="ital">EFGH</span> is greater than the half of the circle <span class="ital">EFGH</span>. </p>

<p>Now let there be set up on the square <span class="ital">EFGH</span> a pyramid having the same vertex with the cone; therefore the pyramid so set up is greater than the half part of the cone. <pb n="411"/></p>

<p>Let the circumferences <span class="ital">EF</span>, <span class="ital">FG</span>, <span class="ital">GH</span>, <span class="ital">HE</span> be bisected at the points <span class="ital">P</span>, <span class="ital">Q</span>, <span class="ital">R</span>, <span class="ital">S</span>, and let <span class="ital">EP</span>, <span class="ital">PF</span>, <span class="ital">FQ</span>, <span class="ital">QG</span>, <span class="ital">GR</span>, <span class="ital">RH</span>, <span class="ital">HS</span>, <span class="ital">SE</span> be joined. </p>

<p>Therefore each of the triangles <span class="ital">EPF</span>, <span class="ital">FQG</span>, <span class="ital">GRH</span>, <span class="ital">HSE</span> is also greater than the half part of that segment of the circle <span class="ital">EFGH</span> which is about it. </p>

<p>Now on each of the triangles <span class="ital">EPF</span>, <span class="ital">FQG</span>, <span class="ital">GRH</span>, <span class="ital">HSE</span> let a pyramid be set up having the same vertex with the cone; therefore each of the pyramids so set up is also greater than the half part of that segment of the cone which is about it. </p>

<p>Thus, bisecting the circumferences so left, joining straight lines, setting up on each of the triangles pyramids having the same vertex with the cone, and doing this continually, we shall leave some segments of the cone which will be less than the excess by which the cone <span class="ital">EFGHN</span> exceeds the solid <span class="ital">O</span>. [<a href="/elem.10.1">X. 1</a>] </p>

<p>Let such be left, and let them be the segments on <span class="ital">EP</span>, <span class="ital">PF</span>, <span class="ital">FQ</span>, <span class="ital">QG</span>, <span class="ital">GR</span>, <span class="ital">RH</span>, <span class="ital">HS</span>, <span class="ital">SE</span>; therefore the remainder, the pyramid of which the polygon <span class="ital">EPFQGRHS</span> is the base and the point <span class="ital">N</span> the vertex, is greater than the solid <span class="ital">O</span>. </p>

<p>Let there be also inscribed in the circle <span class="ital">ABCD</span> the polygon <span class="ital">ATBUCVDW</span> similar and similarly situated to the polygon <span class="ital">EPFQGRHS</span>, and let there be set up on the polygon <span class="ital">ATBUCVDW</span> a pyramid having the same vertex with the cone; of the triangles containing the pyramid of which the polygon <span class="ital">ATBUCVDW</span> is the base and the point <span class="ital">L</span> the vertex let <span class="ital">LBT</span> be one, and of the triangles containing the pyramid of which the polygon <span class="ital">EPFQGRHS</span> is the base and the point <span class="ital">N</span> the vertex let <span class="ital">NFP</span> be one; and let <span class="ital">KT</span>, <span class="ital">MP</span> be joined. </p>

<p>Now, since the cone <span class="ital">ABCDL</span> is similar to the cone <span class="ital">EFGHN</span>, therefore, as <span class="ital">BD</span> is to <span class="ital">FH</span>, so is the axis <span class="ital">KL</span> to the axis <span class="ital">MN</span>. [<a href="/elem.11.def.24">XI. Def. 24</a>] <pb n="412"/></p>

<p>But, as <span class="ital">BD</span> is to <span class="ital">FH</span>, so is <span class="ital">BK</span> to <span class="ital">FM</span>; therefore also, as <span class="ital">BK</span> is to <span class="ital">FM</span>, so is <span class="ital">KL</span> to <span class="ital">MN</span>. </p>

<p>And, alternately, as <span class="ital">BK</span> is to <span class="ital">KL</span>, so is <span class="ital">FM</span> to <span class="ital">MN</span>. [<a href="/elem.5.16">V. 16</a>] </p>

<p>And the sides are proportional about equal angles, namely the angles <span class="ital">BKL</span>, <span class="ital">FMN</span>; therefore the triangle <span class="ital">BKL</span> is similar to the triangle <span class="ital">FMN</span>. [<a href="/elem.6.6">VI. 6</a>] </p>

<p>Again, since, as <span class="ital">BK</span> is to <span class="ital">KT</span>, so is <span class="ital">FM</span> to <span class="ital">MP</span>, and they are about equal angles, namely the angles <span class="ital">BKT</span>, <span class="ital">FMP</span>, inasmuch as, whatever part the angle <span class="ital">BKT</span> is of the four right angles at the centre <span class="ital">K</span>, the same part also is the angle <span class="ital">FMP</span> of the four right angles at the centre <span class="ital">M</span>; since then the sides are proportional about equal angles, therefore the triangle <span class="ital">BKT</span> is similar to the triangle <span class="ital">FMP</span>. [<a href="/elem.6.6">VI. 6</a>] </p>

<p>Again, since it was proved that, as <span class="ital">BK</span> is to <span class="ital">KL</span>, so is <span class="ital">FM</span> to <span class="ital">MN</span>, while <span class="ital">BK</span> is equal to <span class="ital">KT</span>, and <span class="ital">FM</span> to <span class="ital">PM</span>, therefore, as <span class="ital">TK</span> is to <span class="ital">KL</span>, so is <span class="ital">PM</span> to <span class="ital">MN</span>; and the sides are proportional about equal angles, namely the angles <span class="ital">TKL</span>, <span class="ital">PMN</span>, for they are right; therefore the triangle <span class="ital">LKT</span> is similar to the triangle <span class="ital">NMP</span>. [<a href="/elem.6.6">VI. 6</a>] </p>

<p>And since, owing to the similarity of the triangles <span class="ital">LKB</span>, <span class="ital">NMF</span>, as <span class="ital">LB</span> is to <span class="ital">BK</span>, so is <span class="ital">NF</span> to <span class="ital">FM</span>, and, owing to the similarity of the triangles <span class="ital">BKT</span>, <span class="ital">FMP</span>, as <span class="ital">KB</span> is to <span class="ital">BT</span>, so is <span class="ital">MF</span> to <span class="ital">FP</span>, therefore, <span class="ital">ex aequali</span>, as <span class="ital">LB</span> is to <span class="ital">BT</span>, so is <span class="ital">NF</span> to <span class="ital">FP</span>. [<a href="/elem.5.22">V. 22</a>] </p>

<p>Again since, owing to the similarity of the triangles <span class="ital">LTK</span>, <span class="ital">NPM</span>, as <span class="ital">LT</span> is to <span class="ital">TK</span>, so is <span class="ital">NP</span> to <span class="ital">PM</span>, and, owing to the similarity of the triangles <span class="ital">TKB</span>, <span class="ital">PMF</span>, as <span class="ital">KT</span> is to <span class="ital">TB</span>, so is <span class="ital">MP</span> to <span class="ital">PF</span>; therefore, <span class="ital">ex aequali</span>, as <span class="ital">LT</span> is to <span class="ital">TB</span>, so is <span class="ital">NP</span> to <span class="ital">PF</span>. [<a href="/elem.5.22">V. 22</a>] <pb n="413"/></p>

<p>But it was also proved that, as <span class="ital">TB</span> is to <span class="ital">BL</span>, so is <span class="ital">PF</span> to <span class="ital">FN</span>. </p>

<p>Therefore, <foreign lang="la">ex aequali</foreign>, as <span class="ital">TL</span> is to <span class="ital">LB</span>, so is <span class="ital">PN</span> to <span class="ital">NF</span>. [<a href="/elem.5.22">V. 22</a>] </p>

<p>Therefore in the triangles <span class="ital">LTB</span>, <span class="ital">NPF</span> the sides are proportional; therefore the triangles <span class="ital">LTB</span>, <span class="ital">NPF</span> are equiangular; [<a href="/elem.6.5">VI. 5</a>] hence they are also similar. [<a href="/elem.6.def.1">VI. Def. I</a>] </p>

<p>Therefore the pyramid of which the triangle <span class="ital">BKT</span> is the base and the point <span class="ital">L</span> the vertex is also similar to the pyramid of which the triangle <span class="ital">FMP</span> is the base and the point <span class="ital">N</span> the vertex, for they are contained by similar planes equal in multitude. [<a href="/elem.11.def.9">XI. Def. 9</a>] </p>

<p>But similar pyramids which have triangular bases are to one another in the triplicate ratio of their corresponding sides. [<a href="/elem.12.8">XII. 8</a>] </p>

<p>Therefore the pyramid <span class="ital">BKTL</span> has to the pyramid <span class="ital">FMPN</span> the ratio triplicate of that which <span class="ital">BK</span> has to <span class="ital">FM</span>. </p>

<p>Similarly, by joining straight lines from <span class="ital">A</span>, <span class="ital">W</span>, <span class="ital">D</span>, <span class="ital">V</span>, <span class="ital">C</span>, <span class="ital">U</span> to <span class="ital">K</span>, and from <span class="ital">E</span>, <span class="ital">S</span>, <span class="ital">H</span>, <span class="ital">R</span>, <span class="ital">G</span>, <span class="ital">Q</span> to <span class="ital">M</span>, and setting up on each of the triangles pyramids which have the same vertex with the cones, we can prove that each of the similarly arranged pyramids will also have to each similarly arranged pyramid the ratio triplicate of that which the corresponding side <span class="ital">BK</span> has to the corresponding side <span class="ital">FM</span>, that is, which <span class="ital">BD</span> has to <span class="ital">FH</span>. </p>

<p>And, as one of the antecedents is to one of the consequents, so are all the antecedents to all the consequents; [<a href="/elem.5.12">V. 12</a>] therefore also, as the pyramid <span class="ital">BKTL</span> is to the pyramid <span class="ital">FMPN</span>, so is the whole pyramid of which the polygon <span class="ital">ATBUCVDW</span> is the base and the point <span class="ital">L</span> the vertex to the whole pyramid of which the polygon <span class="ital">EPFQGRHS</span> is the base and the point <span class="ital">N</span> the vertex; hence also the pyramid of which <span class="ital">ATBUCVDW</span> is the base and the point <span class="ital">L</span> the vertex has to the pyramid of which the polygon <span class="ital">EPFQGRHS</span> is the base and the point <span class="ital">N</span> the vertex the ratio triplicate of that which <span class="ital">BD</span> has to <span class="ital">FH</span>. </p>

<p>But, by hypothesis, the cone of which the circle <span class="ital">ABCD</span>
       <pb n="414"/>is the base and the point <span class="ital">L</span> the vertex has also to the solid <span class="ital">O</span> the ratio triplicate of that which <span class="ital">BD</span> has to <span class="ital">FH</span>; therefore, as the cone of which the circle <span class="ital">ABCD</span> is the base and the point <span class="ital">L</span> the vertex is to the solid <span class="ital">O</span>, so is the pyramid of which the polygon <span class="ital">ATBUCVDW</span> is the base and <span class="ital">L</span> the vertex to the pyramid of which the polygon <span class="ital">EPFQGRHS</span> is the base and the point <span class="ital">N</span> the vertex; therefore, alternately, as the cone of which the circle <span class="ital">ABCD</span> is the base and <span class="ital">L</span> the vertex is to the pyramid contained in it of which the polygon <span class="ital">ATBUCVDW</span> is the base and <span class="ital">L</span> the vertex, so is the solid <span class="ital">O</span> to the pyramid of which the polygon <span class="ital">EPFQGRHS</span> is the base and <span class="ital">N</span> the vertex. [<a href="/elem.5.16">V. 16</a>] </p>

<p>But the said cone is greater than the pyramid in it; for it encloses it. </p>

<p>Therefore the solid <span class="ital">O</span> is also greater than the pyramid of which the polygon <span class="ital">EPFQGRHS</span> is the base and <span class="ital">N</span> the vertex. </p>

<p>But it is also less: which is impossible. </p>

<p>Therefore the cone of which the circle <span class="ital">ABCD</span> is the base and <span class="ital">L</span> the vertex has not to any solid less than the cone of which the circle <span class="ital">EFGH</span> is the base and the point <span class="ital">N</span> the vertex the ratio triplicate of that which <span class="ital">BD</span> has to <span class="ital">FH</span>: </p>

<p>Similarly we can prove that neither has the cone <span class="ital">EFGHN</span> to any solid less than the cone <span class="ital">ABCDL</span> the ratio triplicate of that which <span class="ital">FH</span> has to <span class="ital">BD</span>. </p>

<p>I say next that neither has the cone <span class="ital">ABCDL</span> to any solid greater than the cone <span class="ital">EFGHN</span> the ratio triplicate of that which <span class="ital">BD</span> has to <span class="ital">FH</span>. </p>

<p>For, if possible, let it have that ratio to a greater solid <span class="ital">O</span>. </p>

<p>Therefore, inversely, the solid <span class="ital">O</span> has to the cone <span class="ital">ABCDL</span> the ratio triplicate of that which <span class="ital">FH</span> has to <span class="ital">BD</span>. </p>

<p>But, as the solid <span class="ital">O</span> is to the cone <span class="ital">ABCDL</span>, so is the cone <span class="ital">EFGHN</span> to some solid less than the cone <span class="ital">ABCDL</span>. </p>

<p>Therefore the cone <span class="ital">EFGHN</span> also has to some solid less than the cone <span class="ital">ABCDL</span> the ratio triplicate of that which <span class="ital">FH</span> has to <span class="ital">BD</span>: which was proved impossible. <pb n="415"/></p>

<p>Therefore the cone <span class="ital">ABCDL</span> has not to any solid greater than the cone <span class="ital">EFGHN</span> the ratio triplicate of that which <span class="ital">BD</span> has to <span class="ital">FH</span>. </p>

<p>But it was proved that neither has it this ratio to a less solid than the cone <span class="ital">EFGHN</span>. </p>

<p>Therefore the cone <span class="ital">ABCDL</span> has to the cone <span class="ital">EFGHN</span> the ratio triplicate of that which <span class="ital">BD</span> has to <span class="ital">FH</span>. </p>

<p>But, as the cone is to the cone, so is the cylinder to the cylinder, for the cylinder which is on the same base as the cone and of equal height with it is triple of the cone; [<a href="/elem.12.10">XII. 10</a>] therefore the cylinder also has to the cylinder the ratio triplicate of that which <span class="ital">BD</span> has to <span class="ital">FH</span>. </p>

<p>Therefore etc. Q. E. D.</p>
