---
title:  Proposition 12.9
subtitle: 
author:
routes:
  aliases:
    - /elem.12.9
collection:
  name: elements
  showCount: true
  showMenu: true
content:
  items: '@self.children'
child_type: article
figure:
  image:
  alt:
  title:
  caption:
taxonomy:
  tag:
  category:
    - 
---

<p>
       <hi rend="ital">In equal pyramids which have triangular bases the bases are reciprocally proportional to the heights; and those pyramids in which the bases are reciprocally proportional to the heights are equal.</hi>
      </p>

===

<p>
       <span class="ital">In equal pyramids which have triangular bases the bases are reciprocally proportional to the heights; and those pyramids in which the bases are reciprocally proportional to the heights are equal.</span>
      </p>

<p>For let there be equal pyramids which have the triangular bases <span class="ital">ABC</span>, <span class="ital">DEF</span> and vertices the points <span class="ital">G</span>, <span class="ital">H</span>; I say that in the pyramids <span class="ital">ABCG</span>, <span class="ital">DEFH</span> the bases are reciprocally proportional to the heights, that is, as the base <span class="ital">ABC</span> is to the base <span class="ital">DEF</span>, so is the height of the pyramid <span class="ital">DEFH</span> to the height of the pyramid <span class="ital">ABCG</span>. 
      </p>

<p>For let the parallelepipedal solids <span class="ital">BGML</span>, <span class="ital">EHQP</span> be completed. </p>

<p>Now, since the pyramid <span class="ital">ABCG</span> is equal to the pyramid <span class="ital">DEFH</span>, and the solid <span class="ital">BGML</span> is six times the pyramid <span class="ital">ABCG</span>, and the solid <span class="ital">EHQP</span> six times the pyramid <span class="ital">DEFH</span>, therefore the solid <span class="ital">BGML</span> is equal to the solid <span class="ital">EHQP</span>. </p>

<p>But in equal parallelepipedal solids the bases are reciprocally proportional to the heights; [<a href="/elem.11.34">XI. 34</a>] therefore, as the base <span class="ital">BM</span> is to the base <span class="ital">EQ</span>, so is the height of the solid <span class="ital">EHQP</span> to the height of the solid <span class="ital">BGML</span>. </p>

<p>But, as the base <span class="ital">BM</span> is to <span class="ital">EQ</span>, so is the triangle <span class="ital">ABC</span> to the triangle <span class="ital">DEF</span>. [<a href="/elem.1.34">I. 34</a>] </p>

<p>Therefore also, as the triangle <span class="ital">ABC</span> is to the triangle <span class="ital">DEF</span>, so is the height of the solid <span class="ital">EHQP</span> to the height of the solid <span class="ital">BGML</span>. [<a href="/elem.5.11">V. 11</a>] <pb n="399"/></p>

<p>But the height of the solid <span class="ital">EHQP</span> is the same with the height of the pyramid <span class="ital">DEFH</span>, and the height of the solid <span class="ital">BGML</span> is the same with the height of the pyramid <span class="ital">ABCG</span>, therefore, as the base <span class="ital">ABC</span> is to the base <span class="ital">DEF</span>, so is the height of the pyramid <span class="ital">DEFH</span> to the height of the pyramid <span class="ital">ABCG</span>. </p>

<p>Therefore in the pyramids <span class="ital">ABCG</span>, <span class="ital">DEFH</span> the bases are reciprocally proportional to the heights. </p>

<p>Next, in the pyramids <span class="ital">ABCG</span>, <span class="ital">DEFH</span> let the bases be reciprocally proportional to the heights; that is, as the base <span class="ital">ABC</span> is to the base <span class="ital">DEF</span>, so let the height of the pyramid <span class="ital">DEFH</span> be to the height of the pyramid <span class="ital">ABCG</span>; I say that the pyramid <span class="ital">ABCG</span> is equal to the pyramid <span class="ital">DEFH</span>. </p>

<p>For, with the same construction, since, as the base <span class="ital">ABC</span> is to the base <span class="ital">DEF</span>, so is the height of the pyramid <span class="ital">DEFH</span> to the height of the pyramid <span class="ital">ABCG</span>, while, as the base <span class="ital">ABC</span> is to the base <span class="ital">DEF</span>, so is the parallelogram <span class="ital">BM</span> to the parallelogram <span class="ital">EQ</span>, therefore also, as the parallelogram <span class="ital">BM</span> is to the parallelogram <span class="ital">EQ</span>, so is the height of the pyramid <span class="ital">DEFH</span> to the height of the pyramid <span class="ital">ABCG</span>. [<a href="/elem.5.11">V. 11</a>] </p>

<p>But the height of the pyramid <span class="ital">DEFH</span> is the same with the height of the parallelepiped <span class="ital">EHQP</span>, and the height of the pyramid <span class="ital">ABCG</span> is the same with the height of the parallelepiped <span class="ital">BGML</span>; therefore, as the base <span class="ital">BM</span> is to the base <span class="ital">EQ</span>, so is the height of the parallelepiped <span class="ital">EHQP</span> to the height of the parallelepiped <span class="ital">BGML</span>. </p>

<p>But those parallelepipedal solids in which the bases are reciprocally proportional to the heights are equal; [<a href="/elem.11.34">XI. 34</a>] therefore the parallelepipedal solid <span class="ital">BGML</span> is equal to the parallelepipedal solid <span class="ital">EHQP</span>. </p>

<p>And the pyramid <span class="ital">ABCG</span> is a sixth part of <span class="ital">BGML</span>, and the pyramid <span class="ital">DEFH</span> a sixth part of the parallelepiped <span class="ital">EHQP</span>; <pb n="400"/>therefore the pyramid <span class="ital">ABCG</span> is equal to the pyramid <span class="ital">DEFH</span>. </p>

<p>Therefore etc Q. E. D.</p>
