---
title:  Proposition 13.7
subtitle: 
author:
routes:
  aliases:
    - /elem.13.7
collection:
  name: elements
  showCount: true
  showMenu: true
content:
  items: '@self.children'
child_type: article
figure:
  image:
  alt:
  title:
  caption:
taxonomy:
  tag:
  category:
    - 
---

<p><hi rend="ital">If three angles of an equilateral pentagon, taken either in order or not in order</hi>, <hi rend="ital">be equal</hi>, <hi rend="ital">the pentagon will be equiangular.</hi>
      </p>

===

<h1>PROPOSITION 7.</h1>
<p><span class="ital">If three angles of an equilateral pentagon, taken either in order or not in order</span>, <span class="ital">be equal</span>, <span class="ital">the pentagon will be equiangular.</span>
      </p>

<p>For in the equilateral pentagon <span class="ital">ABCDE</span> let, first, three angles taken in order, those at <span class="ital">A</span>, <span class="ital">B</span>, <span class="ital">C</span>, be equal to one another; I say that the pentagon <span class="ital">ABCDE</span> is equiangular. 
      </p>

<p>For let <span class="ital">AC</span>, <span class="ital">BE</span>, <span class="ital">FD</span> be joined. </p>

<p>Now, since the two sides <span class="ital">CB</span>, <span class="ital">BA</span> are equal to the two sides <span class="ital">BA</span>, <span class="ital">AE</span> respectively, and the angle <span class="ital">CBA</span> is equal to the angle <span class="ital">BAE</span>, therefore the base <span class="ital">AC</span> is equal to the base <span class="ital">BE</span>, the triangle <span class="ital">ABC</span> is equal to the triangle <span class="ital">ABE</span>, and the remaining angles will be equal to the remaining angles, namely those which the equal sides subtend, [<a href="/elem.1.4">I. 4</a>] that is, the angle <span class="ital">BCA</span> to the angle <span class="ital">BEA</span>, and the angle <span class="ital">ABE</span> to the angle <span class="ital">CAB</span>; hence the side <span class="ital">AF</span> is also equal to the side <span class="ital">BF</span>. [<a href="/elem.1.6">I. 6</a>] <pb n="452"/></p>

<p>But the whole <span class="ital">AC</span> was also proved equal to the whole <span class="ital">BE</span>; therefore the remainder <span class="ital">FC</span> is also equal to the remainder <span class="ital">FE</span>. </p>

<p>But <span class="ital">CD</span> is also equal to <span class="ital">DE</span>. </p>

<p>Therefore the two sides <span class="ital">FC</span>, <span class="ital">CD</span> are equal to the two sides <span class="ital">FE</span>, <span class="ital">ED</span>; and the base <span class="ital">FD</span> is common to them; therefore the angle <span class="ital">FCD</span> is equal to the angle <span class="ital">FED</span>. [<a href="/elem.1.8">I. 8</a>] </p>

<p>But the angle <span class="ital">BCA</span> was also proved equal to the angle <span class="ital">AEB</span>; therefore the whole angle <span class="ital">BCD</span> is also equal to the whole angle <span class="ital">AED</span>. </p>

<p>But, by hypothesis, the angle <span class="ital">BCD</span> is equal to the angles at <span class="ital">A</span>, <span class="ital">B</span>; therefore the angle <span class="ital">AED</span> is also equal to the angles at <span class="ital">A</span>, <span class="ital">B</span>. </p>

<p>Similarly we can prove that the angle <span class="ital">CDE</span> is also equal to the angles at <span class="ital">A</span>, <span class="ital">B</span>, <span class="ital">C</span>; therefore the pentagon <span class="ital">ABCDE</span> is equiangular. </p>

<p>Next, let the given equal angles not be angles taken in order, but let the angles at the points <span class="ital">A</span>, <span class="ital">C</span>, <span class="ital">D</span> be equal; I say that in this case too the pentagon <span class="ital">ABCDE</span> is equiangular. </p>

<p>For let <span class="ital">BD</span> be joined. </p>

<p>Then, since the two sides <span class="ital">BA</span>, <span class="ital">AE</span> are equal to the two sides <span class="ital">BC</span>, <span class="ital">CD</span>, and they contain equal angles, therefore the base <span class="ital">BE</span> is equal to the base <span class="ital">BD</span>, the triangle <span class="ital">ABE</span> is equal to the triangle <span class="ital">BCD</span>, and the remaining angles will be equal to the remaining angles, namely those which the equal sides subtend; [<a href="/elem.1.4">I. 4</a>] therefore the angle <span class="ital">AEB</span> is equal to the angle <span class="ital">CDB</span>. </p>

<p>But the angle <span class="ital">BED</span> is also equal to the angle <span class="ital">BDE</span>, since the side <span class="ital">BE</span> is also equal to the side <span class="ital">BD</span>. [<a href="/elem.1.5">I. 5</a>] </p>

<p>Therefore the whole angle <span class="ital">AED</span> is equal to the whole angle <span class="ital">CDE</span>. </p>

<p>But the angle <span class="ital">CDE</span> is, by hypothesis, equal to the angles at <span class="ital">A</span>, <span class="ital">C</span>; therefore the angle <span class="ital">AED</span> is also equal to the angles at <span class="ital">A</span>, <span class="ital">C</span>. <pb n="453"/></p>

<p>For the same reason the angle <span class="ital">ABC</span> is also equal to the angles at <span class="ital">A</span>, <span class="ital">C</span>, <span class="ital">D</span>. </p>

<p>Therefore the pentagon <span class="ital">ABCDE</span> is equiangular. Q. E. D.</p>
