---
title:  Proposition 8.11
subtitle: 
author:
routes:
  aliases:
    - /elem.8.11
collection:
  name: elements
  showCount: true
  showMenu: true
content:
  items: '@self.children'
child_type: article
figure:
  image:
  alt:
  title:
  caption:
taxonomy:
  tag:
  category:
    - 
---

<p>
       <hi rend="ital">Between two square numbers there is one mean proportional number, and the square has to the square the ratio duplicate of that which the side has to the side.</hi>
      </p>

===

<p>
       <span class="ital">Between two square numbers there is one mean proportional number, and the square has to the square the ratio duplicate of that which the side has to the side.</span>
      </p>

<p>Let <span class="ital">A</span>, <span class="ital">B</span> be square numbers, and let <span class="ital">C</span> be the side of <span class="ital">A</span>, and <span class="ital">D</span> of <span class="ital">B</span>; I say that between <span class="ital">A</span>, <span class="ital">B</span> there is one mean proportional number, and <span class="ital">A</span> has to <span class="ital">B</span> the ratio duplicate of that which <span class="ital">C</span> has to <span class="ital">D</span>. </p>

<p>For let <span class="ital">C</span> by multiplying <span class="ital">D</span> make <span class="ital">E</span>. 
      </p>

<p>Now, since <span class="ital">A</span> is a square and <span class="ital">C</span> is its side, therefore <span class="ital">C</span> by multiplying itself has made <span class="ital">A</span>. </p>

<p>For the same reason also <span class="ital">D</span> by multiplying itself has made <span class="ital">B</span>. </p>

<p>Since then <span class="ital">C</span> by multiplying the numbers <span class="ital">C</span>, <span class="ital">D</span> has made <span class="ital">A</span>, <span class="ital">E</span> respectively, therefore, as <span class="ital">C</span> is to <span class="ital">D</span>, so is <span class="ital">A</span> to <span class="ital">E</span>. [<a href="/elem.7.17">VII. 17</a>] </p>

<p>For the same reason also, <span class="center">as <span class="ital">C</span> is to <span class="ital">D</span>, so is <span class="ital">E</span> to <span class="ital">B</span>. [<a href="/elem.7.18">VII. 18</a>]</span>
      </p>

<p>Therefore also, as <span class="ital">A</span> is to <span class="ital">E</span>, so is <span class="ital">E</span> to <span class="ital">B</span>. </p>

<p>Therefore between <span class="ital">A</span>, <span class="ital">B</span> there is one mean proportional number. </p>

<p>I say next that <span class="ital">A</span> also has to <span class="ital">B</span> the ratio duplicate of that which <span class="ital">C</span> has to <span class="ital">D</span>. </p>

<p>For, since <span class="ital">A</span>, <span class="ital">E</span>, <span class="ital">B</span> are three numbers in proportion, therefore <span class="ital">A</span> has to <span class="ital">B</span> the ratio duplicate of that which <span class="ital">A</span> has to <span class="ital">E</span>. [<a href="/elem.5.def.9">V. Def. 9</a>] </p>

<p>But, as <span class="ital">A</span> is to <span class="ital">E</span>, so is <span class="ital">C</span> to <span class="ital">D</span>. </p>

<p>Therefore <span class="ital">A</span> has to <span class="ital">B</span> the ratio duplicate of that which the side <span class="ital">C</span> has to <span class="ital">D</span>. Q. E. D.</p>
